Constructor description generation done

theories/generator/desc.v
@@ -32,8 +32,6 @@ End MyRepsTypes.
 Module MyReps := Reps MyRepsTypes.
 Import MyReps MyRepsTypes.
 
-Print MyReps.
-
 (* Warning: MetaCoq doesn't use the Monad notation from ExtLib,
   therefore don't expect ExtLib functions to work with TemplateMonad. *)
 Import monad_utils.MonadNotation
@@ -73,24 +71,29 @@ Definition get_representableM {A : Type} : TemplateMonad representable_X :=
     ret (@get_representable A ins)
   end.
 
-
-Inductive code :=
+(* The type to represent a constructor in an inductive data type.
+   The name [reific] stands for "reified inductive constructor".
+   Notice how this type uses Gallina binders,
+   it is a weak HOAS description of the constructor.
+ *)
+Inductive reific :=
 (* the type parameters in parametric polymorphism, isn't represented immediately in memory,
 but the possibility for representation is needed later, e.g., A in [list A]
  *)
- | TYPEPARAM  : (forall (A : Type) `{Rep A}, code) -> code
+ | TYPEPARAM  : (forall (A : Type) `{Rep A}, reific) -> reific
 (* Non-type parameters of a fixed type which isn't represented in memory, e.g., n in [n < m] *)
- | PARAM  : forall A : Type, (A -> code) -> code
+ | PARAM  : forall A : Type, (A -> reific) -> reific
 (* index, represented in memory, e.g. the index of a vector *)
- | INDEX  : forall (A : Type) `{Rep A}, (A -> code) -> code
+ | INDEX  : forall (A : Type) `{Rep A}, (A -> reific) -> reific
  (* non-dependent version of arguments, argument represented in memory, e.g. for X/list X of cons *)
- | ARG : forall (A : Type) `{Rep A}, code -> code
+ | ARG : forall (A : Type) `{Rep A}, reific -> reific
  (* dependent argument, represented in memory, e.g. in positive_nat_list *)
- | DEPARG : forall (A : Type) `{Rep A}, (A -> code) -> code
+ | DEPARG : forall (A : Type) `{Rep A}, (A -> reific) -> reific
 (* the end type, e.g., list X for cons : forall X, X -> list X -> **list X** *)
- | RES  : forall (A : Type) `{Rep A}, code.
+ | RES  : forall (A : Type) `{Rep A}, reific.
 
-Fixpoint args (c : code) : Type :=
+(* Makes nested sigmas (i.e. dependent tuples) of all the arguments. *)
+Fixpoint args (c : reific) : Type :=
   match c with
   | TYPEPARAM f => {A : Type & {H : Rep A & args (f A H)}}
   | PARAM A f => {a : A & args (f a) }
@@ -103,7 +106,7 @@ Fixpoint args (c : code) : Type :=
 Definition Reppy := {A : Type & Rep A}.
 
 (* Instance of result type *)
-Fixpoint result (c: code) (xs : args c) : Reppy :=
+Fixpoint result (c: reific) (xs : args c) : Reppy :=
   match c as l return (args l -> Reppy) with
   | TYPEPARAM f => fun P => let '(a; (h; rest)) := P in result (f a h) rest
   | PARAM A f => fun P => let '(a; rest) := P in result (f a) rest
@@ -113,10 +116,17 @@ Fixpoint result (c: code) (xs : args c) : Reppy :=
   | RES A H => fun _ => (A; H)
   end xs.
 
-Definition reconstruct (c : code) : Type :=
+(* Makes a Coq level constructor type from a [reific], with the new type
+   taking a nested dependent tuple instead of curried arguments. *)
+Definition reconstruct (c : reific) : Type :=
   forall (P : args c),
   let '(A; _) := result c P in A.
 
+(* The same thing as [reconstruct] but takes the actual constructor
+   as an argument but "ignores" it. In reality that argument is
+   used by the tactic to infer how to reconstruct. *)
+Definition reconstructor {T : Type} (x : T) (c : reific) :=
+  reconstruct c.
 
 Ltac destruct_through C :=
   match goal with
@@ -138,37 +148,40 @@ Ltac reconstructing_aux C :=
   intro P;
   destruct_through C.
 
-Definition reconstructor {T : Type} (x : T) (c : code) :=
-  reconstruct c.
-
+(* The entry point to the tactic that solves
+   goals like [reconstructor S S_reific]. *)
 Ltac reconstructing :=
   match goal with
   | [ |- reconstructor ?C _ ] => simpl; reconstructing_aux C
   end.
 
 
-
 (* EXAMPLES *)
-Definition Rep_nat : Rep nat.
+
+(*
+Instance Rep_unit : Rep unit.
   constructor. intros. exact True. Defined.
-Definition Rep_list : forall A : Type, Rep A -> Rep (list A).
+Instance Rep_nat : Rep nat.
+  constructor. intros. exact True. Defined.
+Instance Rep_list : forall A : Type, Rep A -> Rep (list A).
   intros. constructor. intros. exact True. Defined.
+*)
 
 Inductive vec (A : Type) : nat -> Type :=
 | vnil : vec A 0
 | vcons : forall n : nat, A -> vec A n -> vec A (S n).
-Definition Rep_vec : forall (A : Type) (n : nat), Rep A -> Rep (vec A n).
+Instance Rep_vec : forall (A : Type) (n : nat), Rep A -> Rep (vec A n).
   intros. constructor. intros. exact True. Defined.
 
-Definition S_code : code :=
+Definition S_reific : reific :=
   @ARG nat Rep_nat (@RES nat Rep_nat).
 
-Definition cons_code : code :=
+Definition cons_reific : reific :=
   @TYPEPARAM (fun A H =>
                 @ARG A H
                      (@ARG (list A) (Rep_list A H)
                            (@RES (list A) (Rep_list A H)))).
-Goal reconstructor (@cons) cons_code.
+Goal reconstructor (@cons) cons_reific.
   reconstructing. Defined.
 
 Inductive two (A : Type) : Type :=
@@ -178,160 +191,166 @@ Definition Rep_two : forall (A : Type), Rep A -> Rep (two A).
   intros. constructor. intros. exact True. Defined.
 Existing Instance Rep_two.
 
-Definition mkTwo_code : code :=
+Definition mkTwo_reific : reific :=
   @TYPEPARAM (fun A H =>
                 @ARG A H (@ARG A H (@RES (two A) (Rep_two A H)))).
 
-Goal reconstructor mkTwo mkTwo_code.
+Goal reconstructor mkTwo mkTwo_reific.
   reconstructing. Defined.
 
-Definition vcons_code : code :=
+Definition vnil_reific : reific :=
   @TYPEPARAM (fun A H =>
-                @INDEX nat Rep_nat (fun n =>
-                                      @ARG A H (@ARG (vec A n) (Rep_vec A n H)
-                                                     (@RES (vec A (S n)) (Rep_vec A (S n) H))))).
-Goal (reconstructor vcons vcons_code).
+                (@RES (vec A O) (Rep_vec A O H))).
+
+Goal (reconstructor vnil vnil_reific).
   reconstructing. Defined.
 
+Definition vcons_reific : reific :=
+  @TYPEPARAM (fun A H =>
+     @INDEX nat Rep_nat (fun n =>
+       @ARG A H (@ARG (vec A n) (Rep_vec A n H)
+          (@RES (vec A (S n)) (Rep_vec A (S n) H))))).
+
+Goal (reconstructor vcons vcons_reific).
+  reconstructing. Defined.
+
+Check <%% vec %%>.
 
 (* GENERATION *)
 Record constructor_description :=
 { ctor_name : ident;
-  ctor_code : code;
-  ctor_real : reconstruct ctor_code
+  ctor_reific : reific;
+  ctor_real : reconstruct ctor_reific
 }.
-
-Check <%% le %%>.
 
 Definition Reppyish := option ({A : Type & Rep A}).
 
-Axiom TODO : Type.
+Fixpoint adjust_context (ctx : list (ident * Reppyish)) : TemplateMonad (list (ident * named_term)) :=
+  match ctx with
+  | nil => ret nil
+  | (id, None) :: xs => adjust_context xs
+  | (id, Some (A; H)) :: xs =>
+      A' <- tmQuote A ;;
+      xs' <- adjust_context xs ;;
+      ret ((id, A') :: xs')
+  end.
 
-Definition create_code
+Definition kleisli_compose {m a b c} `{Monad m} : (b -> m c) -> (a -> m b) -> (a -> m c) :=
+  fun g f x => f x >>= g.
+
+Definition fresh_aname (prefix : string) (a : aname) : TemplateMonad (ident * aname) :=
+  let x := match binder_name a with | nAnon => prefix | nNamed i => prefix ++ i end in
+  x' <- tmFreshName x ;;
+  ret (x, {| binder_name := nNamed x'; binder_relevance := binder_relevance a |}).
+
+Definition fill_hole
+           (named_ctx : list (ident * named_term))
+           (goal : named_term)
+            : TemplateMonad named_term :=
+  (* quantify all the free variables in the goal *)
+  let quantified : global_term :=
+      fold_left
+        (fun tm '(id, ty) => tProd (mkBindAnn (nNamed id) Relevant) ty tm)
+        named_ctx goal in
+  (* use primitives to infer the type class instance over the global term *)
+  hoisted <- MyReps.instance_term quantified ;;
+  (* make function application again to have the same free variables *)
+  ret (tApp hoisted (rev (map (fun '(id, _) => tVar id) named_ctx))).
+
+(*
+MetaCoq Run (fill_hole [("H", tApp <% Rep %> [tVar "a"]);("a", <% Type %>)]
+                       (tApp <% Rep %> [tApp <% @list %> [tVar "a"]]) >>= tmEval all >>= tmPrint).
+*)
+
+Definition create_reific
+           (ind : inductive)
            (mut : mutual_inductive_body)
            (one : one_inductive_body)
-           (ctor : (ident * term * nat)) : TemplateMonad code :=
+           (ctor : (ident * term * nat)) : TemplateMonad reific :=
   let '(cn, t, arity) := ctor in
-  let fix params (xs : context)
-                 (base : list (ident * Reppyish) -> code)
-                 (ctx : list (ident * Reppyish))
-                 : code :=
-    match xs with
-    | nil => base ctx
-    | x :: rest =>
-      let n := match binder_name (decl_name x) with
-               | nNamed id => id
-               | _ => "_" end in
-      TYPEPARAM (fun r H => params rest base ((n, Some (r; H)) :: ctx))
-    end
+  (* We convert the constructor type to the named representation *)
+  let init_index_ctx : list (ident  * named_term) :=
+      mapi (fun i one => (ind_name one, tInd {| inductive_mind := inductive_mind ind
+                                              ; inductive_ind := i |} []))
+           (ind_bodies mut) in
+  t' <- DB.undeBruijn' (map (fun '(id, _) => nNamed id) init_index_ctx) t ;;
+
+  let fix go
+           (* type of the constructor to be taken apart *)
+             (t : named_term)
+           (* the context kept for De Bruijn indices *)
+             (index_ctx : list (ident  * named_term))
+           (* the context kept for "lambda lifting" the holes *)
+             (named_ctx : list (ident * named_term))
+           (* unprocessed number of parameters left on the type *)
+             (num_params : nat) : TemplateMonad named_term :=
+      match t, num_params with
+      | tProd n (tSort s as t) b , S n' =>
+        '(h, H) <- fresh_aname "H" n ;;
+        let named_ctx' : list (ident * named_term) :=
+            match binder_name n with
+            | nNamed id => (h, tApp <% @Rep %> [tVar id]) :: (id, t) :: named_ctx
+            | _ => named_ctx end in
+        rest <- go b index_ctx named_ctx' (pred num_params) ;;
+        let f := tLambda n (tSort s) (tLambda H (tApp <% @Rep %> [tRel 0]) rest) in
+        ret (tApp <% @TYPEPARAM %> [f])
+
+      | tProd n t b , 0 =>
+        let named_ctx' : list (ident * named_term) :=
+            match binder_name n with
+            | nNamed id => (id, t) :: named_ctx
+            | _ => named_ctx end in
+        rest <- go b index_ctx named_ctx' 0 ;;
+        let t' := Substitution.named_subst_all index_ctx t in
+        let f := tLambda n t' rest in
+        H <- fill_hole named_ctx (tApp <% Rep %> [t']) ;;
+        ret (tApp <% @DEPARG %> [t'; H; f])
+
+      | rest , _ =>
+        let rest' := Substitution.named_subst_all index_ctx rest in
+        H <- fill_hole named_ctx (tApp <% Rep %> [rest']) ;;
+        ret (tApp <% @RES %> [rest'; H])
+      end
   in
 
-  ind_ty (* named_term *) <- DB.undeBruijn (ind_type one) ;;
-
-  let fix indices
-          (t : named_term) (remaining_params : nat) (count : nat)
-          (base : list (ident * Reppyish) -> code)
-          (ctx : list (ident * Reppyish))
-          : code :=
-    match t with
-    | tProd (mkBindAnn nAnon rel) ty rest =>
-      if remaining_params then
-        indices rest (pred remaining_params) count base ctx
-      else
-        PARAM TODO (fun r =>
-          let new_name := "P" ++ string_of_nat count in
-          indices rest (pred remaining_params) (S count) base ((new_name, None) :: ctx))
-    | tProd (mkBindAnn (nNamed id) rel) ty rest =>
-      if remaining_params then
-        indices rest (pred remaining_params) count base ctx
-      else
-        PARAM TODO (fun r =>
-          indices rest (pred remaining_params) (S count) base ((id, None) :: ctx))
-    | _ => base ctx
-    end in
   let num_of_params := ind_npars mut in
-
-  let fix args (t : named_term) (ctx : list (ident * Reppyish)) : code :=
-    @RES Type Rep_Type (* TODO *)
-  in
-  t' <- DB.undeBruijn' nil t ;;
-  let c := params (ind_params mut) (indices ind_ty num_of_params 0 (args t')) in
-  ret (c nil).
-
+  c <- go t' init_index_ctx [] num_of_params ;;
+  c' <- DB.deBruijn c ;;
+  tmUnquoteTyped reific c'.
 
 Definition create_desc {T : Type} (ctor_val : T) : TemplateMonad constructor_description :=
   t <- tmQuote ctor_val ;;
   match t with
-  | tConstruct {| inductive_mind := kn ; inductive_ind := mut_tag |} ctor_tag _ =>
+  | tConstruct ({| inductive_mind := kn ; inductive_ind := mut_tag |} as ind) ctor_tag _ =>
     mut <- tmQuoteInductive kn ;;
 
     match (nth_error (ind_bodies mut) mut_tag) with
     | None => tmFail "Impossible mutual block index"
     | Some one =>
-      tmPrint one ;;
       match (nth_error (ind_ctors one) ctor_tag) with
       | None => tmFail "Impossible constructor index"
       | Some (ctor_name, ctor_type, ctor_arity) =>
-        code <- create_code mut one (ctor_name, ctor_type, ctor_arity) ;;
+        reific <- create_reific ind mut one (ctor_name, ctor_type, ctor_arity) ;;
 
         newName <- tmFreshName "new"%string ;;
-        actual <- tmLemma newName (reconstructor ctor_val code) ;;
+        actual <- tmLemma newName (reconstructor ctor_val reific) ;;
 
         ret {| ctor_name := ctor_name
-             ; ctor_code := code
+             ; ctor_reific := reific
              ; ctor_real := actual
              |}
       end
     end
   | t' => tmPrint t' ;; tmFail "Not a constructor"
-  (* | t' => tmPrint t' ;; tmMsg "error" ;; tmFail "" *)
   end.
 
 Notation "$ x" :=
-  ((ltac:(let p y := exact y in run_template_program (create_desc x) p)))
+  ((ltac:(let p y := exact y in run_template_program (@create_desc _ x) p)))
   (only parsing, at level 30).
 
-MetaCoq Run (create_desc (@Some)).
-Next Obligation.
-  reconstructing_aux (@Some).
-Defined.
+Obligation Tactic := reconstructing.
 
-MetaCoq Run (@create_desc (nat -> option nat) (@Some)).
-Next Obligation.
-  Admitted.
-
-
-Check $ (@le_n).
-Check $ (@le_S).
-Check <%% @nil %%>.
-
-
-
-(* Inductive arg_description := *)
-(* | TYPEPARAM : forall (A : Type) (Rep_A : Rep A), arg_description -> arg_description *)
-(* | PARAM : forall (A : Type) (Rep_A : Rep A), arg_description -> arg_description *)
-(* | INDEX : forall (A : Type) (Rep_A : Rep A), arg_description -> arg_description *)
-(* | ARG : forall (A : Type) (Rep_A : Rep A), arg_description -> arg_description *)
-(* | RES : forall (A : Type) (Rep_A : Rep A), arg_description. *)
-
-
-(* Check *)
-(*    TYPEPARAM (A : Type) (!!Rep_A : Rep A) *)
-(*      (INDEX (n : nat) (!!Rep_n : Rep nat) *)
-(*        (ARG (x : A) (Rep_x : Rep A) *)
-(*          (ARG (xs : vec A n) (Rep_xs : Rep (vec A n) *)
-(*            (RES (vec A (S n)) (@vcons A n x xs) (Rep_res : Rep (vec A (S n)))))))). *)
-
-
-(* Require Import Coq.Program.Equality. *)
-(* Definition test : forall (A : Type) (P1 : nat) (x : vec A P1), Prop. *)
-(* intros. *)
-(* remember x as x'. *)
-(* dependent induction x. *)
-(* exact False. *)
-(* apply (IHx x). auto. *)
-(* Defined. *)
-
-(* Eval compute in test. *)
-
-(* Search _ (vec _ _). *)
+MetaCoq Run (create_desc tt >>= tmPrint).
+MetaCoq Run (create_desc S >>= tmPrint).
+MetaCoq Run (create_desc (@Some) >>= tmPrint).
+MetaCoq Run (create_desc (@cons) >>= tmPrint).
